knefnelkm

LeanGrow/Src/Caching/Formating/Process.lean
@@ -40,16 +40,47 @@ def parseEqIff (goal : Expr) : Option (Bool × Expr × Expr) :=
       .none
 
 
+def badUni? (goal : Expr) (hyps : Array HypType) (sinks : List Nat) : badUniType :=
+  let gdeps := (goal.collectMVars {}).result
+  sinks.foldl (fun S s =>
+    let T := hyps[s]!.type.getAppFn'
+    match T with
+    | .mvar mvid =>
+      match S with
+      | .both => S
+      | .no => if gdeps.contains mvid then .fwdOnly else .both
+      | .fwdOnly => if gdeps.contains mvid then S else .both
+      | .bckOnly => if gdeps.contains mvid then .fwdOnly else .both
+      -- bckOnly not needed :(
+    | _ => S
+    ) .no
+
+def badUniRW? (goal : Expr) (hyps : Array HypType) (sinks : List Nat) : badUniType :=
+  let gdeps := (goal.collectMVars {}).result
+  sinks.foldl (fun S s =>
+    let T := hyps[s]!.type.getAppFn'
+    match T with
+    | .mvar mvid =>
+      match S with
+      | .both => S
+      | .no => if gdeps.contains mvid then S else .both
+      | .fwdOnly => if gdeps.contains mvid then S else .both
+      | .bckOnly => if gdeps.contains mvid then S else .both
+      -- bckOnly not needed :(
+    | _ => S
+    ) .no
+
+
 /-- Bool in output is true if its an rw-thm which has a sink not in the goal-/
 partial def processForMain (l1 : LocalContext) (l2 : LocalInstances)
   (module : Name) (thmIdx : Nat)
   (thmName : Name ⊕ FVarId) (lvlC : Array (LMVarId × Nat)) (lvlN : Nat) (T : Expr)
-  : MetaM (Prod4 Bool (List ThmFormat) LocalContext LocalInstances) :=
+  : MetaM (Prod4 Bool (ListProd badUniType ThmFormat) LocalContext LocalInstances) :=
   do
   let rec go (l1 : LocalContext) (l2 : LocalInstances)
     (hyps : Array HypType) (decls : Array (MVarId × MetavarDecl)) (userNames : Array (Name × MVarId))
     (type : Expr) (pos : Nat) (sinkCand : List (Nat × Nat))
-    : MetaM (Prod4 Bool (List ThmFormat) LocalContext LocalInstances) := do
+    : MetaM (Prod4 Bool (ListProd badUniType ThmFormat) LocalContext LocalInstances) := do
     match type with
     | .letE _ _ V B _ => do
         go l1 l2 hyps decls userNames (Expr.instantiate1 B V) pos sinkCand
@@ -80,55 +111,58 @@ partial def processForMain (l1 : LocalContext) (l2 : LocalInstances)
         | _ =>
           let sinkCand := sinkCand.mergeSort (fun x y => x.2 ≥ y.2)
           -- *note* we sort the sinks by decreasing number of dependencies
+          let sinks := (sinkCand.map Prod.fst)
           match parseEqIff goal with
           | .none =>
               match goal.getAppFn' with
-              | .mvar .. => return .mk false [] l1 l2
+              | .mvar .. => return .mk false .nil l1 l2
               | _ =>
+                let badu := badUni? goal hyps sinks
                 let .mk l1 l2 ← badnessTestPrep l1 l2 module thmIdx hyps
                 let pred? ← IsProp goal l1 l2
-                let sinks := (sinkCand.map Prod.fst)
                 let bf ← isBadForForw l1 l2 sinks hyps goal
                 let bb ← isBadForBack l1 l2 sinks hyps goal
                 let res : ThmFormat :=
                   .std thmName lvlN pred? hyps ⟨lvlC, decls, userNames⟩ hyps.size goal sinks bf bb
-                return .mk false [res] l1 l2
+                return .mk false (.cons badu res .nil) l1 l2
           | .some (iff?, left, right) =>
               let .mk l1 l2 ← badnessTestPrep l1 l2 module thmIdx hyps
               let goalDeps := goal.getLnodePos
-              let sinks := (sinkCand.map Prod.fst)
               let sinksNotInGoal? := sinks.any (fun x => !(goalDeps.contains x))
               let left ← withTransparency .instances <| reduce left
               let right ← withTransparency .instances <| reduce right
               if left == right
               then
-                return .mk sinksNotInGoal? [] l1 l2
+                return .mk sinksNotInGoal? .nil l1 l2
               else
                 match left.getAppFn', right.getAppFn' with
                 | .mvar _, .mvar _ =>
-                    return .mk sinksNotInGoal? [] l1 l2
+                    return .mk sinksNotInGoal? .nil l1 l2
                 | .mvar .., _ =>
                     let .mk bf l1 l2 ← isBadForForwRW l1 l2 right left
                     let .mk bb l1 l2 ← isBadForBackRW l1 l2 sinks hyps right left
                     let .mk si l1 l2 ← simplifierScore l1 l2 right left
+                    let badu := badUniRW? right hyps sinks
                     let resS : ThmFormat :=
                       .rw thmName lvlN (if iff? then .iff_mpr else .eq_mpr)
                           right left hyps ⟨lvlC, decls, userNames⟩ hyps.size sinks
                           bf bb si
-                    return .mk sinksNotInGoal? [resS] l1 l2
+                    return .mk sinksNotInGoal? (.cons badu resS .nil) l1 l2
                 | _, .mvar .. =>
                     let .mk bf l1 l2 ← isBadForForwRW l1 l2 left right
                     let .mk bb l1 l2 ← isBadForBackRW l1 l2 sinks hyps left right
                     let .mk si l1 l2 ← simplifierScore l1 l2 left right
+                    let badu := badUniRW? left hyps sinks
                     let resN : ThmFormat :=
                       .rw thmName lvlN (if iff? then .iff_mp else .eq_mp)
                           left right hyps ⟨lvlC, decls, userNames⟩ hyps.size sinks
                           bf bb si
-                    return .mk sinksNotInGoal? [resN] l1 l2
+                    return .mk sinksNotInGoal? (.cons badu resN .nil) l1 l2
                 | _, _ =>
                     let .mk bf l1 l2 ← isBadForForwRW l1 l2 left right
                     let .mk bb l1 l2 ← isBadForBackRW l1 l2 sinks hyps left right
                     let .mk si l1 l2 ← simplifierScore l1 l2 left right
+                    let baduN := badUniRW? left hyps sinks
                     let resN : ThmFormat :=
                       .rw thmName lvlN (if iff? then .iff_mp else .eq_mp)
                           left right hyps ⟨lvlC, decls, userNames⟩ hyps.size sinks
@@ -136,11 +170,12 @@ partial def processForMain (l1 : LocalContext) (l2 : LocalInstances)
                     let .mk bf l1 l2 ← isBadForForwRW l1 l2 right left
                     let .mk bb l1 l2 ← isBadForBackRW l1 l2 sinks hyps right left
                     let .mk si l1 l2 ← simplifierScore l1 l2 right left
+                    let baduS := badUniRW? right hyps sinks
                     let resS : ThmFormat :=
                       .rw thmName lvlN (if iff? then .iff_mpr else .eq_mpr)
                           right left hyps ⟨lvlC, decls, userNames⟩ hyps.size sinks
                           bf bb si
-                    return .mk sinksNotInGoal? [resN,resS] l1 l2
+                    return .mk sinksNotInGoal? ((.cons baduS resS (.cons baduN resN .nil))) l1 l2
   go l1 l2 #[] #[] #[] T 0 []
 
 
@@ -150,7 +185,7 @@ partial def processForMain (l1 : LocalContext) (l2 : LocalInstances)
 -/
 def processForCache
   (module : Name) (thmIdx : Nat) (cinfo : ConstantInfo)
-  : MetaM (Prod4 Bool (List ThmFormat) LocalContext LocalInstances) :=
+  : MetaM (Prod4 Bool (ListProd badUniType ThmFormat) LocalContext LocalInstances) :=
   do
   let (lvlC,lvlN,T) ← levelsForCache module thmIdx cinfo
   processForMain {} {} module thmIdx (.inl cinfo.name) lvlC lvlN T
@@ -160,7 +195,7 @@ def processForCache
 - list may be empty for such cases
 -/
 def processForQuery (l1 : LocalContext) (l2 : LocalInstances)
-  (gnodeIdx : Nat) (type : Expr) : MetaM (Prod4 Bool (List ThmFormat) LocalContext LocalInstances) :=
+  (gnodeIdx : Nat) (type : Expr) : MetaM (Prod4 Bool (ListProd badUniType ThmFormat) LocalContext LocalInstances) :=
   do
   processForMain l1 l2 `processForQuery gnodeIdx (.inr <| ⟨gnode gnodeIdx⟩) #[] 0 type
 
@@ -169,13 +204,13 @@ def processForQuery (l1 : LocalContext) (l2 : LocalInstances)
 -/
 partial def processForCacheSpe
   (module : Name) (thmIdx : Nat) (cinfo : ConstantInfo)
-  : MetaM (Prod4 Bool (List ThmFormat) LocalContext LocalInstances) := do
+  : MetaM (Prod4 Bool (ListProd badUniType ThmFormat) LocalContext LocalInstances) := do
   let thmName := (.inl cinfo.name)
   let (lvlC,lvlN,T) ← levelsForCache module thmIdx cinfo
   let rec go (l1 : LocalContext) (l2 : LocalInstances)
     (hyps : Array HypType) (decls : Array (MVarId × MetavarDecl)) (userNames : Array (Name × MVarId))
     (type : Expr) (pos : Nat) (sinkCand : List (Nat × Nat))
-    : MetaM (Prod4 Bool (List ThmFormat) LocalContext LocalInstances) := do
+    : MetaM (Prod4 Bool (ListProd badUniType ThmFormat) LocalContext LocalInstances) := do
     match type with
     | .letE _ _ V B _ => do
         go l1 l2 hyps decls userNames (Expr.instantiate1 B V) pos sinkCand
@@ -209,9 +244,10 @@ partial def processForCacheSpe
           let .mk l1 l2 ← badnessTestPrep l1 l2 module thmIdx hyps
           let pred? ← IsProp goal l1 l2
           let sinks := (sinkCand.map Prod.fst)
+          let badu := badUni? goal hyps sinks
           let bf ← isBadForForw l1 l2 sinks hyps goal
           let bb ← isBadForBack l1 l2 sinks hyps goal
           let res : ThmFormat :=
             .std thmName lvlN pred? hyps ⟨lvlC, decls, userNames⟩ hyps.size goal sinks bf bb
-          return .mk false [res] l1 l2
+          return .mk false (.cons badu res .nil) l1 l2
   go {} {} #[] #[] #[] T 0 []
