LeanGrow/Src/Caching/Query/Build.lean
@@ -1,0 +1,280 @@
+
+/-
+Copyright (c) 2025 Yves Jäckle. All rights reserved.
+Released under Apache 2.0 license as described in the file LICENSE.
+Author: Yves Jäckle.
+-/
+
+import LeanGrow.Src.Caching.Formating.Process
+import LeanGrow.Src.Caching.Query.PaInGMergeSpe
+import LeanGrow.Src.Utils.Lean.ImportExport
+import LeanGrow.Src.Utils.Std.Name
+import LeanGrow.Src.Utils.Lean.Blacklisting
+
+open Lean Meta
+
+variable {IdxCollType : Type _}
+
+
+structure ModuleCacheState (IdxCollType : Type _) where
+  thm_data : Array ThmFormat
+  thmNameToIdx : CTrie (List Nat)
+  thmNameToHypIdx : CTrie (List Nat)
+  stdBackPaIn : PaInG IdxCollType
+  stdForwSetTrie : SetTrieP ThmFormat IdxCollType PaInG
+  stdForwSetTrie_idxToThmIdx : Array Nat
+  rwBackPaIn : PaInG IdxCollType
+  rwForwPaIn : PaInG IdxCollType
+deriving Inhabited
+
+structure ModuleCacheStatePartial (IdxCollType : Type _) where
+  Cstop : Nat
+  countThm : Nat
+  countHyps : Nat
+  thm_data : Array ThmFormat
+  thmNameToIdx : CTrie (List Nat)
+  thmNameToHypIdx : CTrie (List Nat)
+  stdBackPaIn : PaInG IdxCollType
+  stdForwSetTrie : ListProd (PaInG IdxCollType) ThmFormat
+  stdForwSetTrie_idxToThmIdx : Array Nat
+  rwBackPaIn : PaInG IdxCollType
+  rwForwPaIn : PaInG IdxCollType
+deriving Inhabited
+
+
+-- #exit
+
+@[specialize, inline]
+partial def buildCachDataForCore [Repr IdxCollType]
+  (emptyCol : IdxCollType)
+  (singleton : Nat → IdxCollType) (insert : Nat → IdxCollType → IdxCollType)
+  (module : Name) (cinfos : Array ConstantInfo) (Cstart Cstop : Nat)
+  (sofarBack : PaInG IdxCollType) (formats : Array ThmFormat)
+  (sofarBackRW : PaInG IdxCollType) (countThm : Nat) (sofarFwd : ListProd (PaInG IdxCollType) ThmFormat)
+  (hyptothm : Array Nat) (sofarFwdRW : PaInG IdxCollType) (countHyps : Nat) (thmNameToIdx thmNameToHypIdx : CTrie (List Nat))
+  : MetaM (ModuleCacheStatePartial IdxCollType) :=
+  let rec @[specialize] inner (ciN : ByteArray)
+    (sofarBack : PaInG IdxCollType) (formats : Array ThmFormat)
+    (sofarBackRW : PaInG IdxCollType) (countThm : Nat) (sofarFwd : ListProd (PaInG IdxCollType) ThmFormat)
+    (hyptothm : Array Nat) (sofarFwdRW : PaInG IdxCollType) (countHyps : Nat) (thmNameToIdx thmNameToHypIdx : CTrie (List Nat))
+    (rwWithSinkNotInGoal : Bool) (data : ListProd badUniType ThmFormat)
+    : MetaM (Prod10 _ _ _ _ _ _ _ _ _ _) := do
+    mtracing
+    match data with
+    | .nil =>
+        return .mk sofarBack formats sofarBackRW countThm sofarFwd hyptothm sofarFwdRW countHyps thmNameToIdx thmNameToHypIdx
+    | .cons badu d@(.std _ _ _ hyps _ _ goal sinks ..) more =>
+        mtrace on .zero with s!" std case"
+        mtrace on .zero with s!" badu {repr badu}"
+        mtrace on .one with s!" sinks {sinks}"
+        match badu with
+        | .both =>
+          inner ciN sofarBack formats sofarBackRW countThm sofarFwd hyptothm sofarFwdRW countHyps thmNameToIdx thmNameToHypIdx rwWithSinkNotInGoal more
+        | .fwdOnly =>
+          let formats := formats.push d
+          let ⟨sofarBack,_,_⟩ ← sofarBack.insert (← getLCtx) (← getLocalInstances) goal countThm emptyCol singleton insert
+          mtrace on .zero with s!" add goal to back"
+          -- let ciN := cinfo.name.toString.toUTF8
+          let thmNameToIdx := thmNameToIdx.insert ciN [countThm]
+          let countThm := countThm + 1
+          inner ciN sofarBack formats sofarBackRW countThm sofarFwd hyptothm sofarFwdRW countHyps thmNameToIdx thmNameToHypIdx rwWithSinkNotInGoal more
+        | .bckOnly =>
+          let formats := formats.push d
+          let HforFwdPaIn := sinks.foldl (fun S s => match hyps[s]! with | .inst .. => S | .reg type => (type) :: S) []
+          let (FwdPaIn,_) ← HforFwdPaIn.foldlM (fun (T,i) e => do
+            let ⟨res,_,_⟩ ← T.insert (← getLCtx) (← getLocalInstances) e i emptyCol singleton insert
+            mtrace on .zero with s!" for forw, added hyp {← ppExpr e}"
+            return (res, i+1)) (PaInG.dead, countHyps)
+          let sofarFwd := .cons FwdPaIn d sofarFwd
+          let hyptothm := (hyptothm.pushN countThm) HforFwdPaIn.length
+          -- let ciN := cinfo.name.toString.toUTF8
+          let thmNameToIdx := thmNameToIdx.insert ciN [countThm]
+          let countThm := countThm + 1
+          let thmNameToHypIdx := thmNameToHypIdx.insert ciN (List.Ico countHyps (countHyps + HforFwdPaIn.length))
+          let countHyps := countHyps + HforFwdPaIn.length
+          inner ciN sofarBack formats sofarBackRW countThm sofarFwd hyptothm sofarFwdRW countHyps thmNameToIdx thmNameToHypIdx rwWithSinkNotInGoal more
+        | .no =>
+          let formats := formats.push d
+          let ⟨sofarBack,_,_⟩ ← sofarBack.insert (← getLCtx) (← getLocalInstances) goal countThm emptyCol singleton insert
+          mtrace on .zero with s!" add goal to back"
+          let HforFwdPaIn := sinks.foldl (fun S s => match hyps[s]! with | .inst .. => S | .reg type => (type) :: S) []
+          let (FwdPaIn,_) ← HforFwdPaIn.foldlM (fun (T,i) e => do
+            let ⟨res,_,_⟩ ← T.insert (← getLCtx) (← getLocalInstances) e i emptyCol singleton insert
+            mtrace on .zero with s!" for forw, added hyp {← ppExpr e}"
+            return (res, i+1)) (PaInG.dead, countHyps)
+          let sofarFwd := .cons FwdPaIn d sofarFwd
+          let hyptothm := (hyptothm.pushN countThm) HforFwdPaIn.length
+          -- let ciN := cinfo.name.toString.toUTF8
+          let thmNameToIdx := thmNameToIdx.insert ciN [countThm]
+          let countThm := countThm + 1
+          let thmNameToHypIdx := thmNameToHypIdx.insert ciN (List.Ico countHyps (countHyps + HforFwdPaIn.length))
+          let countHyps := countHyps + HforFwdPaIn.length
+          inner ciN sofarBack formats sofarBackRW countThm sofarFwd hyptothm sofarFwdRW countHyps thmNameToIdx thmNameToHypIdx rwWithSinkNotInGoal more
+    | .cons badu fst@(.rw _ _ _ goal ..) more => do
+        mtrace on .zero with s!" rw case"
+        mtrace on .zero with s!" badu {repr badu}"
+        match badu with
+        | .no =>
+          let formats := (formats.push fst)
+          mtrace on .zero with s!" rwWithSinkNotInGoal {rwWithSinkNotInGoal} "
+          if !rwWithSinkNotInGoal
+          then
+            let ⟨sofarBackRW,_,_⟩ ← sofarBackRW.insert (← getLCtx) (← getLocalInstances) goal countThm emptyCol singleton insert
+            mtrace on .zero with s!" added left to back"
+            let ⟨sofarFwdRW,_,_⟩ ← sofarFwdRW.insert (← getLCtx) (← getLocalInstances) goal countThm emptyCol singleton insert
+            mtrace on .zero with s!" added left to forw"
+            let thmNameToIdx := thmNameToIdx.insert ciN [countThm]
+            let countThm := countThm + 1
+            inner ciN sofarBack formats sofarBackRW countThm sofarFwd hyptothm sofarFwdRW countHyps thmNameToIdx thmNameToHypIdx rwWithSinkNotInGoal more
+          else
+            let ⟨sofarBackRW,_,_⟩ ← sofarBackRW.insert (← getLCtx) (← getLocalInstances) goal countThm emptyCol singleton insert
+            mtrace on .zero with s!" added left to back"
+            let thmNameToIdx := thmNameToIdx.insert ciN [countThm]
+            let countThm := countThm + 1
+            inner ciN sofarBack formats sofarBackRW countThm sofarFwd hyptothm sofarFwdRW countHyps thmNameToIdx thmNameToHypIdx rwWithSinkNotInGoal more
+        | _ =>
+          inner ciN sofarBack formats sofarBackRW countThm sofarFwd hyptothm sofarFwdRW countHyps thmNameToIdx thmNameToHypIdx rwWithSinkNotInGoal more
+  let rec @[specialize] go (cinfoI : Nat) (sofarBack : PaInG IdxCollType) (formats : Array ThmFormat)
+    (sofarBackRW : PaInG IdxCollType) (countThm : Nat) (sofarFwd : ListProd (PaInG IdxCollType) ThmFormat)
+    (hyptothm : Array Nat) (sofarFwdRW : PaInG IdxCollType) (countHyps : Nat) (thmNameToIdx thmNameToHypIdx : CTrie (List Nat))
+    : MetaM (ModuleCacheStatePartial IdxCollType) := do
+    mtracing
+    if cinfoI ≥ cinfos.size || cinfoI ≥ Cstop
+    then
+      let final : ModuleCacheStatePartial IdxCollType :=
+          {Cstop := Cstop
+           countThm := countThm
+           countHyps := countHyps
+           thm_data := formats
+           thmNameToIdx := thmNameToIdx
+           thmNameToHypIdx := thmNameToHypIdx
+           stdBackPaIn := sofarBack
+           stdForwSetTrie := sofarFwd
+           stdForwSetTrie_idxToThmIdx := hyptothm
+           rwBackPaIn := sofarBackRW
+           rwForwPaIn := sofarFwdRW
+          }
+      return final
+    else
+      let cinfo := cinfos[cinfoI]!
+      mtrace on .zero with s!" on decl {cinfo.name} with idx {countThm}"
+      if cinfo.name.blackListCaching (← getEnv)
+      then
+        mtrace on .zero with s!" blacklisted !"
+        go (cinfoI + 1) sofarBack formats sofarBackRW countThm sofarFwd hyptothm sofarFwdRW countHyps thmNameToIdx thmNameToHypIdx
+      else
+        let .mk rwWithSinkNotInGoal data _ _ ← processForCache module countThm cinfo
+        mtrace on .zero with s!" passed processForCache"
+        let ciN := cinfo.name.toString.toUTF8
+        let .mk sofarBack formats sofarBackRW countThm sofarFwd hyptothm sofarFwdRW countHyps thmNameToIdx thmNameToHypIdx ← inner ciN sofarBack formats sofarBackRW countThm sofarFwd hyptothm sofarFwdRW countHyps thmNameToIdx thmNameToHypIdx rwWithSinkNotInGoal data
+        go (cinfoI + 1) sofarBack formats sofarBackRW countThm sofarFwd hyptothm sofarFwdRW countHyps thmNameToIdx thmNameToHypIdx
+  Meta.withUnlimitedHeartbeats do
+  mtracing
+  mtrace on .zero with s!" unlimited heartbeats"
+  Meta.withResetRecDepth do
+    mtrace on .zero with s!" reset rec depth"
+    go Cstart sofarBack formats sofarBackRW countThm sofarFwd hyptothm sofarFwdRW countHyps thmNameToIdx thmNameToHypIdx
+
+-- #exit
+
+def LeanGrow.mkCacheName : Name → String :=
+  (fun n => s!"LeanGrow_ThmFormatQueryCache{n.toUnderscoreString}")
+
+def LeanGrow.mkPartialCacheName : Name → String :=
+  (fun n => s!"LeanGrow_ThmFormatQueryPartialCache{n.toUnderscoreString}")
+
+#print Import
+
+open System
+
+@[specialize, inline]
+unsafe def buildPartialCacheData [Repr IdxCollType]
+  (emptyCol : IdxCollType)
+  (singleton : Nat → IdxCollType) (insert : Nat → IdxCollType → IdxCollType)
+  (modules : Array Name) (StepSize : Nat) (opts : Options := {}) : IO Unit :=
+  withImportModules (modules.map (fun x => {module := x})) opts <| fun env => do
+    stdMetaRun env do
+      let cachePath ← findLeanGrowCacheDir
+      let finalPath := FilePath.join cachePath (FilePath.toString "withUnpickleTracing.txt")
+      let mut regs : Array CompactedRegion := Array.replicate modules.size (0 : USize)
+      let mut i := 0
+      for module in modules do
+        let path := FilePath.join cachePath ⟨LeanGrow.mkPartialCacheName module⟩
+        if !(← path.pathExists)
+        then
+          let .some midx := env.getModuleIdx? module | throwError s!"[buildCachData] unknonw module {module}"
+          let cinfos := (env.header.moduleData[midx]!).constants
+          let res ← buildCachDataForCore emptyCol singleton insert
+                      module cinfos
+                      0 StepSize
+                      .dead #[] .dead 0 .nil #[] .dead 0 .empty .empty
+          let finalPath := FilePath.join cachePath (FilePath.toString (LeanGrow.mkPartialCacheName module))
+          pickle finalPath res
+          i := i+1
+        else
+          let (x, region) ← unpickle (ModuleCacheStatePartial IdxCollType) path
+          regs := regs.set! i region
+          let .some midx := env.getModuleIdx? module | throwError s!"[buildCachData] unknonw module {module}"
+          let cinfos := (env.header.moduleData[midx]!).constants
+          if x.Cstop ≥ cinfos.size
+          then
+            throwError s!"[buildCachData] no more steps necessary"
+          else
+            let res ← buildCachDataForCore emptyCol singleton insert
+                        module cinfos
+                        x.Cstop (x.Cstop + StepSize)
+                        x.stdBackPaIn x.thm_data x.rwBackPaIn x.countThm x.stdForwSetTrie  x.stdForwSetTrie_idxToThmIdx x.rwForwPaIn x.countHyps x.thmNameToIdx x.thmNameToHypIdx
+            let finalPath := FilePath.join cachePath (FilePath.toString (LeanGrow.mkPartialCacheName module))
+            pickle finalPath res
+            i := i+1
+      for reg in regs do
+        reg.free
+
+#check 1
+
+
+
+@[specialize, inline]
+unsafe def buildPartialCacheDataS (modules : Array Name) (StepSize : Nat)  (opts : Options := {}) : IO Unit :=
+  buildPartialCacheData
+    UInt32Array.empty (fun x => UInt32Array.single x.toUInt32) (fun x y => y.oInsert x.toUInt32)
+    modules StepSize opts
+
+
+
+@[specialize, inline]
+unsafe def buildCacheData [Repr IdxCollType]
+  (intersect union difference : IdxCollType → IdxCollType → IdxCollType)
+  (emptyCol : IdxCollType) (empty? : IdxCollType → Bool) (size : IdxCollType → Nat)
+  (modules : Array Name) (opts : Options := {}) : IO Unit :=
+  withImportModules (modules.map (fun x => {module := x})) opts <| fun env => do
+    stdMetaRun env do
+
+      let cachePath ← findLeanGrowCacheDir
+      let mut regs : Array CompactedRegion := Array.replicate modules.size (0 : USize)
+      let mut i := 0
+      for module in modules do
+        let path := FilePath.join cachePath ⟨LeanGrow.mkPartialCacheName module⟩
+        let (x, region) ← unpickle (ModuleCacheStatePartial IdxCollType) path
+        regs := regs.set! i region
+        stdImportTracePicklePerImport
+          modules opts
+          LeanGrow.mkCacheName
+          (fun module => do
+            let thmData : CTrie (Array ThmFormat) :=
+              CTrie.insert .empty (module.toString.toUTF8) x.thm_data
+            let res ← SetTriePGSpe.ofList thmData intersect union difference emptyCol empty? size x.stdForwSetTrie
+            let final : ModuleCacheState IdxCollType :=
+              ⟨x.thm_data, x.thmNameToIdx, x.thmNameToHypIdx, x.stdBackPaIn, res, x.stdForwSetTrie_idxToThmIdx, x.rwBackPaIn, x.rwForwPaIn⟩
+            return (final, s!"Cached {module} !")
+            )
+        i := i+1
+      for reg in regs do
+        reg.free
+
+
+@[specialize, inline]
+unsafe def buildCacheDataS (modules : Array Name) (opts : Options := {}) : IO Unit :=
+  buildCacheData
+    (UInt32Array.inter) (UInt32Array.union) (UInt32Array.diff) UInt32Array.empty UInt32Array.isEmpty UInt32Array.size
+    modules opts
