LeanGrow/Src/Caching/Query/PaInGMergeSpe.lean
@@ -7,15 +7,17 @@ Author: Yves Jäckle.
 -/
 
 
-import LeanGrowBeta.Data.PathIndex.Operations
-import LeanGrowBeta.Caching.Formating.Types
+import LeanGrow.Src.Data.PathIndexG.Operations
+import LeanGrow.Src.Caching.Formating.Types
+import LeanGrow.Src.Data.SetTrie.Specialize
+
 
 
 open Lean Meta
 
 variable {IdxCollType : Type _}
 
-namespace PaIn
+namespace PaInG
 
 
 @[specialize, inline]
@@ -25,6 +27,7 @@ private def helpSpe_1 [Repr IdxCollType]
   (union : IdxCollType → IdxCollType → IdxCollType)
   (L R : CTrie (ListProd IdxCollType (Nat × Nat)))
   : MetaM (CTrie (ListProd IdxCollType (Nat × Nat))) := do
+  mtracing
   L.foldMcps R (fun lmod ldata res q0 => do
     let lMod := (String.fromUTF8! lmod).toName
     match thmData.find? lmod with
@@ -32,7 +35,7 @@ private def helpSpe_1 [Repr IdxCollType]
     | .some thms =>
         ldata.foldlMcps res (fun linds (thmIdx,pos) res q1 => do
           mtrace on .zero with s!"[helpSpe_1] left lnode {lMod} {(thmIdx,pos)}, with indices {repr linds}"
-          (thms[thmIdx]!).mctx.load
+          (thms[thmIdx]!).mctx.loadNoCo
           let ln := Expr.mvar ⟨lnode lMod thmIdx pos⟩
           res.foldMcps (Option.none : Option (Nat × Nat)) (fun rmod rdata _ q2 => do
             let rMod := (String.fromUTF8! rmod).toName
@@ -77,8 +80,8 @@ private def helpSpe_1 [Repr IdxCollType]
 partial def mergeLSpeDown [Repr IdxCollType]
   (union : IdxCollType → IdxCollType → IdxCollType)
   (helpSpe : CTrie (ListProd IdxCollType (Nat × Nat)) → CTrie (ListProd IdxCollType (Nat × Nat)) → MetaM (CTrie (ListProd IdxCollType (Nat × Nat))))
-  (A B : PaIn IdxCollType)
-  (sofar : mergeT IdxCollType) (vals : List (PaIn IdxCollType)) : MetaM ((mergeT IdxCollType) × (List (PaIn IdxCollType))) :=
+  (A B : PaInG IdxCollType)
+  (sofar : mergeT IdxCollType) (vals : List (PaInG IdxCollType)) : MetaM ((mergeT IdxCollType) × (List (PaInG IdxCollType))) :=
   let rec debt : List Level → List Level → Bool
     | x :: xs , y :: ys => if x.EqUpToMVar y then debt xs ys else false
     | [], [] => true
@@ -101,16 +104,16 @@ partial def mergeLSpeDown [Repr IdxCollType]
     let lai := (union lai lai')
     let ali := (union ali ali')
     let lei := (union lei lei')
-    let proto : PaIn IdxCollType := .br nt nl ng nu nb ns nc nli
+    let proto : PaInG IdxCollType := .br nt nl ng nu nb ns nc nli
       .dead .dead api .dead .dead lai .dead .dead ali .dead .dead .dead lei
       .empty .dead .dead
     let vals := proto :: vals
     let sofar : mergeT IdxCollType := .proofs proofs proofs' (.sig3 sofar)
     let sofar : mergeT IdxCollType := .proofsOf proofsOf proofsOf' (.sig2 sofar)
     -- todo : optimize ↓
-    let projs : CTrie ((ListProd IdxCollType (Nat × ((PaIn IdxCollType) × (PaIn IdxCollType))))) := projs.map (fun x => .some (x.mapTR (fun x (y,z) => (x,y,z,.dead))))
-    let projs' : CTrie ((ListProd IdxCollType (Nat × ((PaIn IdxCollType) × (PaIn IdxCollType))))) := projs'.map (fun x => .some (x.mapTR (fun x (y,z) => (x,y,.dead,z))))
-    let mproj := @CTrie.merge (ListProd IdxCollType (Nat × ((PaIn IdxCollType) × (PaIn IdxCollType)))) (fun l1 l2 =>
+    let projs : CTrie ((ListProd IdxCollType (Nat × ((PaInG IdxCollType) × (PaInG IdxCollType))))) := projs.map (fun x => .some (x.mapTR (fun x (y,z) => (x,y,z,.dead))))
+    let projs' : CTrie ((ListProd IdxCollType (Nat × ((PaInG IdxCollType) × (PaInG IdxCollType))))) := projs'.map (fun x => .some (x.mapTR (fun x (y,z) => (x,y,.dead,z))))
+    let mproj := @CTrie.merge (ListProd IdxCollType (Nat × ((PaInG IdxCollType) × (PaInG IdxCollType)))) (fun l1 l2 =>
       help_3 union (fun x y => x.1 == y.1) (fun x y => (x.1,x.2.1,y.2.2)) l1 l2
       ) projs projs'
     let sofar : mergeT IdxCollType := mproj.fold sofar (fun bytA L sofar => L.foldl sofar (fun is (i,t1,t2) sofar => .projPre t1 t2 (.projPost bytA i is sofar)))
@@ -131,8 +134,8 @@ partial def mergeLSpeDown [Repr IdxCollType]
 partial def mergeLSpeUp {IdxCollType : Type} [Repr IdxCollType]
   (union : IdxCollType → IdxCollType → IdxCollType) (emptyCol : IdxCollType)
   (helpSpe : CTrie (ListProd IdxCollType (Nat × Nat)) → CTrie (ListProd IdxCollType (Nat × Nat)) → MetaM (CTrie (ListProd IdxCollType (Nat × Nat))))
-  (T : PaIn IdxCollType)
-  (todo : mergeT IdxCollType) (vals : List (PaIn IdxCollType)) : MetaM (PaIn IdxCollType) := do
+  (T : PaInG IdxCollType)
+  (todo : mergeT IdxCollType) (vals : List (PaInG IdxCollType)) : MetaM (PaInG IdxCollType) := do
   match todo with
   | .nil => return T
   | .done T nx => mergeLSpeUp union emptyCol helpSpe T nx vals
@@ -279,7 +282,8 @@ private def helpSpe_2 [Repr IdxCollType]
   (l1 : LocalContext) (l2 : LocalInstances)
   (union : IdxCollType → IdxCollType → IdxCollType)
   (L R : CTrie (ListProd IdxCollType (Nat × Nat)))
-  : MetaM (CTrie (ListProd IdxCollType (Nat × Nat))) :=
+  : MetaM (CTrie (ListProd IdxCollType (Nat × Nat))) := do
+  mtracing
   L.foldMcps R (fun lmod ldata res q0 => do
     let lMod := (String.fromUTF8! lmod).toName
     ldata.foldlMcps res (fun linds (thmIdx,pos) res q1 => do
@@ -328,7 +332,7 @@ partial def mergeLSpe [Repr IdxCollType]
   (union : IdxCollType → IdxCollType → IdxCollType) (emptyCol : IdxCollType)
   (l1 : LocalContext) (l2 : LocalInstances)
   (thmData : CTrie (Array ThmFormat))
-  (A B : PaIn IdxCollType) : MetaM (PaIn IdxCollType) := do
+  (A B : PaInG IdxCollType) : MetaM (PaInG IdxCollType) := do
   let (nx,vals) := ← mergeLSpeDown union (helpSpe_1 l1 l2 thmData union) A B .nil []
   mergeLSpeUp union emptyCol (helpSpe_1 l1 l2 thmData union) .dead nx vals
 
@@ -338,6 +342,41 @@ partial def mergeLSpe [Repr IdxCollType]
 partial def mergeLSpeSpe [Repr IdxCollType]
   (union : IdxCollType → IdxCollType → IdxCollType) (emptyCol : IdxCollType)
   (l1 : LocalContext) (l2 : LocalInstances)
-  (A B : PaIn IdxCollType) : MetaM (PaIn IdxCollType) := do
+  (A B : PaInG IdxCollType) : MetaM (PaInG IdxCollType) := do
   let (nx,vals) := ← mergeLSpeDown union (helpSpe_2 l1 l2 union) A B .nil []
   mergeLSpeUp union emptyCol (helpSpe_2 l1 l2 union) .dead nx vals
+
+end PaInG
+
+@[specialize]
+def SetTriePGSpe.ofList [Inhabited α] [Repr α] [Repr IdxCollType]
+  (thmData : CTrie (Array ThmFormat))
+  (intersect union difference : IdxCollType → IdxCollType → IdxCollType)
+  (emptyCol : IdxCollType)  (empty? : IdxCollType → Bool) (size : IdxCollType → Nat)
+  (l : ListProd (PaInG IdxCollType) α)
+  : MetaM (SetTrieP α IdxCollType PaInG) :=
+  trace set TracingFlags.none in do
+  let res ← SetTrie.ofListMcps
+    (PaInG.dead, PaInG.dead)
+    (fun x (y,z) q => do q (PaInG.merge union emptyCol x y, ← PaInG.mergeLSpe union emptyCol {} {} thmData x z))
+    (fun (x,y) =>
+      trace on .zero with s!"[SetTrieP.ofList] x : {repr x}\n[SetTrieP.ofList] y : {repr y}\n" in
+      match y.max intersect empty? size with
+      | .none => OptionProd.none
+      | .some inds m =>
+          trace on .zero with s!"[SetTrieP.ofList] inds : {repr inds} ; m {m}\n" in
+          let res := x.keepOnlyOfInds inds difference union emptyCol empty?
+          -- ↑ should be buildIndices
+          -- in fact, it should be x with all indices except for inds deleted
+          -- so that we pass a PaIn, that we can use in addKey ↓
+          let is := res.getIndices emptyCol union
+          OptionProd.some (is, res) m
+      )
+    (fun x (is,_) q => q <| x.sharesIndicesWith intersect empty? is)
+    (fun x (is,_) => x.deleteOfInds is difference emptyCol empty?)
+    (fun x => match x.clean emptyCol empty? with | .dead => true | _ => false)
+    (fun (_,es) q =>  q es)
+    (fun (_,es) τ q => q <| PaInG.merge union emptyCol es τ)
+    l
+    (fun x => return x)
+  return SetTrieP.mk (PaInG.merge union emptyCol) .dead (PaInG.getIndices emptyCol union) res
